Use well formedness instead of covers

proof/Poly/Ty.v
@@ -22,77 +22,23 @@ Definition tyenv := env ty.
 Definition kienv := env ki.
 
 
-(* Closedness *******************************************************)
+(* Well Formedness **************************************************)
 
-(* Type is closed under a kind environment of a given length. *)
-Inductive coversTT : nat -> ty -> Prop :=
- | CoversTT_con 
-   :  forall n c
-   ,  coversTT n (TCon c)
-
- | CoversTT_var         
-   :  forall n i
-   ,  n > i 
-   -> coversTT n (TVar i)
-
- | CoversTT_forall
-   :  forall n t
-   ,  coversTT (S n) t
-   -> coversTT n (TForall t)
-
- | CoversT_fun
-   :  forall n t1 t2
-   ,  coversTT n t1 -> coversTT n t2
-   -> coversTT n (TFun t1 t2).
-Hint Constructors coversTT.
-
-
-(* Type is closed under the given kind environment. *)
-Inductive closedUnderTT : kienv -> ty -> Prop :=
- | ClosedUnderTT 
-   :  forall kenv t
-   ,  coversTT (length kenv) t
-   -> closedUnderTT kenv t.
+(* Well formed types are closed under the given kind environment *)
+Fixpoint wfT (kenv: kienv) (tt: ty) : Prop := 
+ match tt with
+ | TCon _     => True
+ | TVar it    => exists k, get kenv it = Some k
+ | TForall t  => wfT (kenv :> KStar) t
+ | TFun t1 t2 => wfT kenv t1 /\ wfT kenv t2
+ end.
+Hint Unfold wfT.
 
 
 (* Type is closed under an empty kind environment. *)
-Inductive closedTT : ty -> Prop :=
- | ClosedTT 
-   :  forall t
-   ,  coversTT 0 t
-   -> closedTT t.
-Hint Constructors closedTT.
+Definition closedT (tt: ty) : Prop
+ := wfT Empty tt.
+Hint Unfold closedT.
 
-
-(* Normal Types *****************************************************
-   A normal form type is a closed type that cannot be reduced further.
- *)
-Inductive normalT : ty -> Prop :=
- | NormalT_con
-   : forall c
-   , normalT (TCon c)
-
- | NormalT_forall
-   :  forall t
-   ,  normalT t
-   -> normalT (TForall t)
-
- | NormalT_fun
-   :  forall t1 t2
-   ,  normalT t1 -> normalT t2
-   -> normalT (TFun t1 t2).
-Hint Constructors normalT.
-
-
-(* Lemmas ***********************************************************)
-Lemma coversTT_succ
- :  forall n t
- ,  coversTT n     t
- -> coversTT (S n) t.
-Proof.
- intros. gen n.
- induction t; intros; inversions H; auto.
-Qed.
-Hint Resolve coversTT_succ.
 
   
